
---

mathLink: auto

---
Date created: 2024-02-11 17:03
Tags: #Type/Theorem #Topic/Real_Analysis 

Proved by: [[Finite series (Properties)]]
References: _Not applicable_
Justifications: [[Infinite series]]

Specializations: _Not applicable_
Generalizations: _Not applicable_

---  

> [!quote] Theorem: Properties of infinite series
> 1. If $\sum^{\infty}_{n=m}a_{n}$ is a series of real numbers converging to $x$ and $\sum^{\infty}_{n=m}b_{n}$ is one converging to $y$ then the series $\sum^{\infty}_{n=m}a_{n}+b_{n}$ is also convergent and converges to $x+y$ in particular $$ \sum^{\infty}_{n=m}a_{n}+b_{n}=\sum^{\infty}_{n=m}a_{n}+\sum^{\infty}_{n=m}b_{n} $$
> 2. If $\sum^{\infty}_{n=m}a_{n}$ is a series of real numbers converging to $x$ and $c$ is any real number, then the series $\sum^{\infty}_{n=m}ca_{n}$ is also convergent and converges to $cx$, in particular we have $$ \sum^{\infty}_{n=m}ca_{n}=c \sum^{\infty}_{n=m}a_{n} $$
> 3. If $\sum^{\infty}_{n=m}a_{n}$ is a series of real numbers and let $k\geq 0$ be an integer. If one of the two series $\sum^{\infty}_{n=m}a_{n}$ and $\sum^{\infty}_{n=m+k}a_{n}$, then the other one is also, and we have the identity $$ \sum^{\infty}_{n=m}a_{n}=\sum^{m+k-1}_{n=m+k}a_{n}+\sum^{\infty}_{n=m+k}a_{n} $$
> 4. If $\sum^{\infty}_{n=m}a_{n}$ is a series of real numbers converging to $x$ and $k$ is some integer then $\sum^{\infty}_{n=m+k}a_{n-k}$ is also convergent and converges to $x$


