---
mathLink: auto
Date created: 2024-09-06 22:26
tags:
  - Type/Theorem
  - Topic/Linear_Algebra
cssclasses:
---

---

Proved by: _Not applicable_
References: _Not applicable_
Justifications: [[Left and right inverse of a matrix]]

Specializations: _Not applicable_
Generalizations: _Not applicable_

---

> [!quote] Theorem:
> Let $A,B\in M_{n\times n}(F)$ be invertible matrices, then 
> - $(A*B)^{-1}=B^{-1}*A^{-1}$
> - $(A^{-1})^{-1}=A$
> - $A^{T}$ is invertible and $(A^{-1})^{T}=(A^{T})^{-1}$
> - If $A$ has a zero row or column then $A$ is not invertible
> - $AD=AC\implies D=C$

