
---

mathLink: auto

---
Date created: 2024-02-26 16:22
Tags: #Type/Theorem  #Topic/Real_Analysis 

Proved by: _Not applicable_
References: [[Rearrangement of series of non-negative reals (Proof)]]
Justifications: [[Infinite series]]

Specializations: _Not applicable_
Generalizations: [[Rearrangement of absolutely converging series]]

---  

> [!quote] Theorem: Rearrangement of series of non-negative reals
>Let $\sum^{\infty}_{n=0}a_{n}$ be a convergent series of non-negative real numbers, and let $f:\mathbb{N} \to \mathbb{N}$ be a bijection. Then $\sum^{\infty}_{m=0}a_{f(m)}$ is also convergent and $$ \sum^{\infty}_{n=0}a_{n}=\sum^{\infty}_{m=0}a_{f(m)} $$



